DS: type check of last protocol step
The type check already includes predicates required to proof the security
properties 'key secrecy', 'replay mitigation' and 'initiator authentication'.
Though, there is still some more work to do to proof the authentication
property (if possible at all).

denning-sacco/DS.Messages.fst
@@ -81,6 +81,27 @@ let parse_encval_comm_key #i #l enc_sig_ck =
 let parse_encval_lemma #i #l enc_sig_ck = ()
 let parse_serialize_encval_lemma #i #l ser_ck sig_ck = ()
 
+let encval_comm_key_publishable_implies_comm_key_publishable i enc_sig_ck =
+  LC.splittable_term_publishable_implies_components_publishable_forall ds_global_usage;
+  split_is_split_len_prefixed enc_sig_ck;
+  match parse_encval_comm_key_ enc_sig_ck with
+  | Success (ser_ck, sig_ck) -> (
+    assert(is_succ2 (split_len_prefixed 4 enc_sig_ck) ser_ck sig_ck);
+    assert(LC.is_publishable ds_global_usage i enc_sig_ck ==> LC.is_publishable ds_global_usage i ser_ck);
+    split_is_split_len_prefixed ser_ck;
+    match parse_sigval_ ser_ck with
+    | Success (CommKey ck t) ->
+      let Success (tag_bytes, rest) = split_len_prefixed 4 ser_ck in
+      assert(is_succ2 (split_len_prefixed 4 ser_ck) tag_bytes rest);
+      assert(LC.is_publishable ds_global_usage i enc_sig_ck ==> LC.is_publishable ds_global_usage i rest);
+      split_is_split_len_prefixed rest;
+      let Success (ck', t_bytes) = split_len_prefixed 4 rest in
+      assert(is_succ2 (split_len_prefixed 4 rest) ck' t_bytes /\ ck' == ck);
+      assert(LC.is_publishable ds_global_usage i enc_sig_ck ==> LC.is_publishable ds_global_usage i ck')
+    | _ -> ()
+  )
+  | _ -> ()
+
 
 let serialize_msg i m =
   match m with
