denning-sacco/DS.Sessions.fsti
@@ -35,7 +35,7 @@ let valid_session (i:nat) (p:principal) (si vi:nat) (st:session_st) =
     (is_comm_key i ck p b \/ LC.corrupt_id i (P srv))
   | ResponderRecvedMsg3 a srv ck ->
     M.is_msg i ck (readers [P p]) /\
-    (is_labeled i ck (join (readers [P a]) (readers [P p])) \/ LC.corrupt_id i (P a) \/ LC.corrupt_id i (P srv))
+    (is_labeled i ck (join (readers [P a]) (readers [P p])) \/ LC.corrupt_id i (P a) \/ LC.corrupt_id i (P srv) \/ LC.is_publishable M.ds_global_usage i ck)
   | _ -> True
 
 let valid_session_later (i j:timestamp) (p:principal) (si vi:nat) (st:session_st) :
@@ -69,7 +69,7 @@ let epred idx s e =
       a = s /\
       clock_cnt <= M.recv_msg_2_delay /\
       (LC.get_sk_label M.ds_key_usages pk_b == readers [P b] /\
-      did_event_occur_before idx srv (M.event_certify a b srv pk_a pk_b t 0) \/ LC.corrupt_id idx (P srv)) /\
+      did_event_occur_at t srv (M.event_certify a b srv pk_a pk_b t 0) \/ LC.corrupt_id idx (P srv)) /\
       was_rand_generated_before idx ck (join (readers [P a]) (LC.get_sk_label M.ds_key_usages pk_b)) (aead_usage "DS.comm_key")
     | _ -> False
   )
@@ -78,8 +78,9 @@ let epred idx s e =
     | (Success a, Success b, Success srv, Success t, Success clock_cnt) ->
       b = s /\
       clock_cnt <= M.recv_msg_3_delay /\
-      ((exists clock_cnt'. clock_cnt' <= M.recv_msg_2_delay /\ did_event_occur_before idx a (M.event_send_key a b srv pk_a pk_b ck t clock_cnt')) \/
-      LC.corrupt_id idx (P a) \/ LC.corrupt_id idx (P srv))
+      ((exists srv' clock_cnt'. clock_cnt' <= M.recv_msg_2_delay /\ did_event_occur_before idx a (M.event_send_key a b srv pk_a pk_b ck t clock_cnt') \/ LC.corrupt_id idx (srv')) /\
+      was_rand_generated_before idx ck (join (readers [P a]) (readers [P b])) (aead_usage "DS.comm_key") \/
+      LC.corrupt_id idx (P a) \/ LC.corrupt_id idx (P srv) \/ LC.is_publishable M.ds_global_usage idx ck)
     | _ -> False
   )
   | _ -> False
